\documentclass{article}
\usepackage{amssymb}

\begin{document}
    \[ \int_{a}^{b}f(x)dx = \lim_{n\to\infty} (\frac{b-a}{n}\sum_{i=0}^{n-1}f(x_i)) \] \bigskip 
    $\int_{a}^{b}f(x)dx = \int_{a}^{c}f(x)dx + \int_{c}^{b}f(x)dx$ \\ \bigskip
    $\int_{a}^{a}f(x)dx = 0$ \\ \bigskip
    The \textbf{average value} of a continuous function \textit{f} for an interval [a,b] is $\frac{1}{b-a}\int_{a}^{b}f(x)dx$ \\ \bigskip
    $y= ax^3-6bx^2-9, $ \\ $ \frac{dy}{dx}= 3ax^2-12bx$ \\ \bigskip
    $y= x^3a-6bx^2-9, $ \\ $ \frac{dy}{da}= x^3 $ \\ \bigskip
    $y= -6x^2b+ax^3-9, $ \\ $ \frac{dy}{db}= -6x^2$ \\
    $\frac{db}{dy} = \frac{1}{\frac{dy}{db}} = -\frac{1}{6x^2} = -6x^{-2}$ \\ \bigskip
    $\frac{dy}{dx} = \frac{dy}{du}\times\frac{du}{dx}$ \\ \bigskip
    $\therefore\frac{dx}{du}\times\frac{du}{dx} = 1$ \\ \bigskip
    $\int f(u)\frac{du}{dx}dx = \int f(u)du$ \\ \smallskip
    $\int f(3x+1)dx$ \\ Let u = 3x+1 \\ \smallskip
    $ = \int f(u)\frac{d(3x+1)}{dx}du$ \\ \smallskip
    $ = \int 3f(u)du$ \\ \bigskip
    \[ \int_{0}^{4} f(x)dx = F(4) - F(0) \] \\ \smallskip
    \[\int_{M}^{N}f(x)dx = -\int_{N}^{M}f(x)dx\]
    \[\int_{M}^{M}f(x)dx = 0\] \bigskip\bigskip\bigskip
    \[\int_{1}^{3}x^2dx=\frac{1}{3}x^3\Big|^3_1=\frac{27}{3}-\frac{1}{3}=8\frac{1}{3}\]
    \end{document}